pcuic/theories/PCUICTyping.v
@@ -832,6 +832,7 @@ Inductive typing `{checker_flags} (Σ : global_context) (Γ : context) : term ->
     Σ ;;; Γ |- tFix mfix n : decl.(dtype)
 
 | type_CoFix mfix n decl :
+    allow_cofix ->
     let types := fix_context mfix in
     nth_error mfix n = Some decl ->
     All_local_env (lift_typing typing Σ) (Γ ,,, types) ->
